Refinement from bit sequences to machine words

refinement/bits.v
@@ -18,289 +18,140 @@ Set Implicit Arguments.
 Unset Strict Implicit.
 Unset Printing Implicit Defensive.
 
+
+
+(**
+
+ The refinement relations have a type of the following form
+
+ <<
+   R : specification -> implementation -> Type
+ >>
+
+  while the transport lemmas have the form
+
+   <<
+     Lemma R_op: refines refinement_relation specification implementation.
+   >>
+
+*)
+
+
 (************************************************************************)
 (** * Refinement Relations                                                 *)
 (************************************************************************)
 
-Parameter w: nat.
+(* XXX: the following refinement are not in the correct order
+(spec/implem): this must be updated. *)
 
+(* 
 
 Definition Rword {n} : 'B_n -> word n -> Type := fun_hrel (@bitw n).
 Definition Rtuple {n} : bitseq -> 'B_n -> Type := fun_hrel val.
 Definition Rbits {n} : bitseq -> word n -> Type := Rtuple \o Rword.
+Definition Rnat: nat -> bitseq -> Type := fun_hrel nats.
 
-Definition Rnat {n} : bitseq -> nat -> Type := fun_hrel (bitn n).
+*)
+
+
+(** ** Refinement from bit sequences to machines words *)
+
+Parameter w: nat.
 
 Module Wordsize.
   Definition wordsize := w.
 End Wordsize.
 Module Native := Make(Wordsize).
 
-Definition Rnative: Native.Int -> bitseq -> Type := Native.Tnative.
-Definition Rnum: Native.Int -> nat -> Type := Rnative \o (@Rnat w).
+Definition Rnative: bitseq -> Native.Int -> Type := fun_hrel (bitsFromInt Native.w).
+
+(* "small" integers (ie. less than the word size) for shifts *)
+CoInductive Ridx: nat -> Native.Int -> Type := 
+  Ridx_spec (n: nat)(i: Native.Int) of 
+    (n <= Native.w)%N
+  & bitsFromInt Native.w i = bitn Native.w n : Ridx n i.
 
 (************************************************************************)
 (** * From machine words to bit sequences                               *)
 (************************************************************************)
 
-(* Pierre: there is a problem with [eq_adj] and the way we deal with [bitseq]s. *)
 
-Section Try.
-
-Import Native.
-Definition NInt_rel (i: Int) (bs: bitseq) : Prop := bs = bitsFromInt w i.
-
-Global Instance eq_Rnative_try:
-  refines (NInt_rel ==> NInt_rel ==> param.bool_R)%rel Native.eq (eqtype.eq_op).
+Global Instance Rnative_eq:
+  refines (Rnative ==> Rnative ==> param.bool_R)%rel (eqtype.eq_op) Native.eq.
 Proof.
-rewrite !refinesE => w1 bs1 -> w2 bs2 ->.
-suff -> : eq w1 w2 = (bitsFromInt w w1 == bitsFromInt w w2).
-  exact: bool_Rxx.
-by apply/eqIntP/eqP => [->//|]; exact: bitsFromInt_inj.
+  rewrite !refinesE => bs1 w1 <- bs2 w2 <-.
+  suff -> : Native.eq w1 w2 = (bitsFromInt w w1 == bitsFromInt w w2)
+    by exact: bool_Rxx.
+  apply/eqIntP/eqP => [->//|]; exact: Native.bitsFromInt_inj.
 Qed.
 
-Global Instance land_Rnative_try:
-  refines (NInt_rel ==> NInt_rel ==> NInt_rel) Native.land ands.
-Proof.
-rewrite !refinesE => w1 bs1 -> w2 bs2 ->.
-have /forallIntP /(_ w1) /forallIntP /(_ w2) /eqIntP -> := land_valid.
-by rewrite /NInt_rel bitsToIntK.
+Global Instance Rnative_zero: refines Rnative '0_w Native.zero.
+Proof. 
+  rewrite refinesE. 
+  have /eqIntP -> := Native.zero_valid.
+  by rewrite /Rnative/fun_hrel Native.bitsToIntK. 
 Qed.
 
-End Try.
-
-(*
-Proof.
-  rewrite refinesE=> i1 bs1 Ribs1 i2 bs2 Ribs2.
-  move: Ribs1 Ribs2.
-  rewrite /eq_op/eq_NativeInt/Rnative/Native.Tnative.
-  rewrite Native.eq_adj.
-  repeat (rewrite Native.eq_adj; move/eqP=> ->).
-  have ->: (NativeInt.eq i1 i2) = (bitsFromInt w i1 == bitsFromInt w i2)
-    by apply/eqIntP/eqP; intro; subst; auto using Native.bitsFromInt_inj.
-  exact: bool_Rxx.
+Global Instance Rnative_one: refines Rnative (bitn w 1) Native.one.
+Proof. 
+  rewrite refinesE. 
+  have /eqIntP -> := Native.one_valid.
+  by rewrite /Rnative/fun_hrel Native.bitsToIntK. 
 Qed.
-*)
 
-Global Instance zero_Rnative: refines Rnative Native.zero '0_w.
-Proof. rewrite refinesE. apply Native.zero_valid. Qed.
-
-Global Instance one_Rnative: refines Rnative Native.one (bitn w 1).
-Proof. rewrite refinesE. apply Native.one_valid. Qed.
-
-Global Instance lnot_Rnative:
-  refines (Rnative ==> Rnative) Native.lnot negs.
-Admitted.
-(*
+Global Instance Rnative_lnot:
+  refines (Rnative ==> Rnative) negs Native.lnot.
 Proof.
-  rewrite refinesE=> i bs.
-  rewrite /Rnative/Native.Tnative Native.eq_adj.
-  move/eqP=> ->.
-  move: i; apply/forallIntP.
-  by apply Native.lnot_valid.
+  rewrite refinesE=> bs w <-.
+  have /forallIntP /(_ w) /eqIntP -> := Native.lnot_valid.
+  by rewrite /Rnative/Native.Tnative/fun_hrel Native.bitsToIntK.
 Qed.
-*)
 
-Global Instance land_Rnative:
-  refines (Rnative ==> Rnative ==> Rnative) Native.land ands.
-Admitted.
-(*
+Global Instance Rnative_land:
+  refines (Rnative ==> Rnative ==> Rnative) ands Native.land.
 Proof.
-  rewrite refinesE=> i1 bs1 Ribs1 i2 bs2 Ribs2. move: Ribs1 Ribs2.
-  repeat (rewrite /Rnative/Native.Tnative Native.eq_adj; move/eqP=> ->).
-  move: i2; apply: forallIntP.
-  move: i1; apply: forallIntP.
-  by apply Native.land_valid.
+  rewrite !refinesE => bs1 w1 <- bs2 w2 <-.
+  have /forallIntP /(_ w1) /forallIntP /(_ w2) /eqIntP -> := Native.land_valid.
+  by rewrite /Rnative/fun_hrel Native.bitsToIntK.
 Qed.
-*)
 
-Global Instance lor_Rnative: 
-  refines (Rnative ==> Rnative ==> Rnative) Native.lor ors.
-Admitted.
-(*
+Global Instance Rnative_lor: 
+  refines (Rnative ==> Rnative ==> Rnative) ors Native.lor.
 Proof.
-  rewrite refinesE=> i1 bs1 Ribs1 i2 bs2 Ribs2.
-  move: Ribs1 Ribs2.
-  repeat (rewrite /Rnative/Native.Tnative Native.eq_adj; move/eqP=> ->).
-  move: i2; apply: forallIntP.
-  move: i1; apply: forallIntP.
-  by apply Native.lor_valid.
+  rewrite !refinesE => bs1 w1 <- bs2 w2 <-.
+  have /forallIntP /(_ w1) /forallIntP /(_ w2) /eqIntP -> := Native.lor_valid.
+  by rewrite /Rnative/fun_hrel Native.bitsToIntK.
 Qed.
-*)
 
-Global Instance lxor_Rnative: 
-  refines (Rnative ==> Rnative ==> Rnative) Native.lxor xors.
-Admitted.
-(*
+Global Instance Rnative_lxor: 
+  refines (Rnative ==> Rnative ==> Rnative) xors Native.lxor.
 Proof.
-  rewrite refinesE=> i1 bs1 Ribs1 i2 bs2 Ribs2.
-  move: Ribs1 Ribs2.
-  repeat (rewrite /Rnative/Native.Tnative Native.eq_adj; move/eqP=> ->).
-  move: i2; apply: forallIntP.
-  move: i1; apply: forallIntP.
-  by apply Native.lxor_valid.
+  rewrite !refinesE => bs1 w1 <- bs2 w2 <-.
+  have /forallIntP /(_ w1) /forallIntP /(_ w2) /eqIntP -> := Native.lxor_valid.
+  by rewrite /Rnative/fun_hrel Native.bitsToIntK.
 Qed.
-*)
 
-(* XXX: explicit bounding of k is not satisfactory. *)
-Global Instance lsr_Rnative: forall k n, (n <= w)%N -> Rnum k n ->
-  refines (Rnative ==> Rnative) (fun i => Native.lsr i k) (fun i => shrs i n).
-Admitted.
-(*
+Global Instance Rnative_lsr: 
+  refines (Rnative ==> Ridx ==> Rnative) shrs Native.lsr.
 Proof.
-  move=> k n Hleq Rkn.
-  rewrite refinesE=> i bs Ribs.
-  move: Rkn Ribs.
-  rewrite /Rnum/Rnat/Rnative/Native.Tnative.
-  rewrite /comp_hrel.
-  move=> [bs2 [/eqIntP Hi2 Hbs2]].
-  rewrite /Rnative/Native.Tnative Native.eq_adj; move/eqP=> ->.
-
-  have Hn: n = nats (bitsFromInt w k).
-  rewrite Hi2.
-  
-  
-  
-  Search bitsFromInt bitsToInt.
-  rewrite Native.eq_adj.
-
-  rewrite <-Hbs2 in Hi2.
-  move/eqIntP: Hi2=> Hi2.
-  rewrite -[NativeInt.eq _ _]/(eq_op _ _) in Hi2.
-  
-  rewrite Hbs2 in Hi2.
-  rewrite eq_adj in Hi2.
-
-
-    := forallInt (fun i =>
-       forallInt (fun i' =>
-         let n := nats (bitsFromInt w i') in
-         (n <= w) ==>
-         Tnative (lsr i i') 
-                 (shrs (bitsFromInt w i) n))).
-
-
-  move/existsP=> [bs' /andP [H /eqP H']].
-  rewrite /Rnative eq_adj in H.
-  move/eqP: H=> H.
-  apply/eqInt32P.
-  have Hk: k = toNat (bitsFromInt32 i').
-    rewrite H.
-    have ->: k = toNat (fromNat (n := wordsize) k).
-      rewrite toNat_fromNatBounded=> //.
-      by apply (leq_ltn_trans (n := wordsize)).
-    by rewrite H'.
-  rewrite Hk.
-  rewrite Hk in ltn_k.
-  clear H H' Hk.
-  move: i' ltn_k; apply/(forallInt32P (fun i' => implb (toNat (bitsFromInt32 i') <= wordsize)%nat (eq (lsr i i') (bitsToInt32 (shrBn (bitsFromInt32 i) (toNat ((bitsFromInt32 i')))))))).
-  move=> i'.
-  apply/equivP.
-  apply/implyP.
-  split=> H H'.
-  move: (H H')=> H''.
-  by apply/eqInt32P.
-  move: (H H')=> H''.
-  by apply/eqInt32P.
-  move: i; apply/forallInt32P; last by apply lsr_valid.
-  move=> i'; apply idP.
+  rewrite !refinesE => bs1 w1 <- _ _ [n i Hn Hi].
+  have H : nats (bitsFromInt Native.w i) = n
+    by rewrite Hi bitnK; 
+       try (eapply leq_ltn_trans, ltn_expl).
+  subst n.
+  have /forallIntP /(_ w1) /forallIntP /(_ i) /implyP /(_ Hn) /eqIntP -> := Native.lsr_valid.
+  by rewrite /Rnative/fun_hrel Native.bitsToIntK.
 Qed.
-*)
 
-(*
 Global Instance lsl_repr: 
-  refines (Rnative ==> Rnative ==> Rnative) <<< (fun x y => shlBn x (toNat y)).
-Admitted.
-(*
+  refines (Rnative ==> Ridx ==> Rnative) shls Native.lsl.
 Proof.
-  move=> i i' ? k ltn_k.
-  rewrite /Rnative eq_adj; move/eqP=> <-.
-  rewrite /natural_repr.
-  move/existsP=> [bs' /andP [H /eqP H']].
-  rewrite /Rnative eq_adj in H.
-  move/eqP: H=> H.
-  apply/eqInt32P.
-  have Hk: k = toNat (bitsFromInt32 i').
-    rewrite H.
-    have ->: k = toNat (fromNat (n := wordsize) k).
-      rewrite toNat_fromNatBounded=> //.
-      by apply (leq_ltn_trans (n := wordsize)).
-    by rewrite H'.
-  rewrite Hk.
-  rewrite Hk in ltn_k.
-  clear H H' Hk.
-  move: i' ltn_k; apply/(forallInt32P (fun i' => implb (toNat (bitsFromInt32 i') <= wordsize)%nat (eq (lsl i i') (bitsToInt32 (shlBn (bitsFromInt32 i) (toNat ((bitsFromInt32 i')))))))).
-  move=> i'.
-  apply/equivP.
-  apply/implyP.
-  split=> H H'.
-  move: (H H')=> H''.
-  by apply/eqInt32P.
-  move: (H H')=> H''.
-  by apply/eqInt32P.
-  move: i; apply/forallInt32P; last by apply lsl_valid.
-  move=> i'; apply idP.
+  rewrite !refinesE => bs1 w1 <- _ _ [n i Hn Hi].
+  have H : nats (bitsFromInt Native.w i) = n
+    by rewrite Hi bitnK; 
+       try (eapply leq_ltn_trans, ltn_expl).
+  subst n.
+  have /forallIntP /(_ w1) /forallIntP /(_ i) /implyP /(_ Hn) /eqIntP -> := Native.lsl_valid.
+  by rewrite /Rnative/fun_hrel Native.bitsToIntK.
 Qed.
-*)
-*)
 
-(************************************************************************)
-(** * Drafts of instances                                               *)
-(************************************************************************)
-
-(* XXX: this must be removed/updated *)
-
-(*
-Axiom W0 : forall n,  word n.+1.
-
-Global Instance zero_Rword {n}: refines Rword (B0 (W0 n).
-Admitted.
-
-Global Instance zero_Rtuple {n}: refines Rtuple '0_n (B0 n).
-Admitted.
-
-Global Instance zero_Rbits {n}: refines Rbits '0_n (W0 n).
-Proof. eapply refines_trans; tc. Qed.
-
-Axiom andw: forall {n}, word n -> word n -> word n.
-Axiom negw: forall {n}, word n -> word n.
-Axiom negBB: forall {n}, 'B_n -> 'B_n.
-
-Global Instance and_Rword {n}: 
-  refines (Rword ==> Rword ==> Rword) (@andB n) andw.
-Admitted.
-
-Global Instance and_Rtuple {n}: 
-  refines (Rtuple ==> Rtuple ==> Rtuple) ands (@andB n).
-Admitted.
-
-Global Instance and_Rbits {n}: 
-  refines (Rbits ==> Rbits ==> Rbits) ands (@andw n).
-Proof. eapply refines_trans; tc. Qed.
-
-
-Section Operations.
-
-Variable (Bits : Type).
-Variable (and : Bits -> Bits -> Bits).
-Variable (not : Bits -> Bits).
-
-Definition nand (bs bs': Bits): Bits 
-  := not (and bs bs').
-
-End Operations.
-
-Parametricity nand.
-
-Check nand_R.
-
-Global Instance neg_Rbits {n}: 
-  refines (Rbits ==> Rbits) negB (@negw n).
-Admitted.
-
-Global Instance nand_Rbits {n}: 
-  refines (Rbits ==> Rbits ==> Rbits) 
-          (@nand _ ands negB) 
-          (@nand _ (@andw n) negw). 
-Proof. param nand_R. Qed.
-*)
